src/tactic/hammer/mex1.lean
@@ -4,4 +4,4 @@ import tactic.hammer.monomorphization data.nat.gcd data.real.basic
 set_option trace.super true
 
 example (x y : ℝ) (h : x < y) : ∃ z : ℚ, x < z ∧ (z : ℝ) < y :=
-by hammer_via_monom 60
+by hammer_via_monom 50
