src/tactic/hammer/mex9.lean
@@ -3,5 +3,5 @@ import tactic.hammer.monomorphization data.nat.gcd data.real.basic
 -- set_option profiler true
 set_option trace.super true
 
-example (x y z : ℕ) : nat.gcd x y ∣ x * z :=
+example (x y z : ℕ) : nat.gcd x y ∣ z * x :=
 by hammer_via_monom
